Add addBindings_typing simp case

LocalLang/TypingGuarantees.lean
@@ -6,10 +6,34 @@ import LocalLang.Typing
 def EnvRespectsCtx (Γ : TypeContext) (V : Env) : Prop :=
   ∀ (x : String) (n : ℕ), V[x]? = some n → Γ[x]? = LLType.nat
 
+def CtxRespectsEnv (V : Env) (Γ : TypeContext) : Prop :=
+  ∀ x : String, Γ[x]? = some LLType.nat → x ∈ V
+
+def CtxRespectsDefs (Γ : TypeContext) (defs : Definitions) : Prop :=
+   (T_ret : LLType) → (arg_types : List LLType) → (f : String) → (f_in_defs : f ∈ defs) →
+    (h_type : Γ[f]? = some (LLType.func arg_types T_ret)) →
+    (TypeJdg Γ defs[f].body T_ret)
+
+
+theorem addBindings_typing {ps : List String} {es : List Expr} {bd : Expr}
+                                {T_ret : LLType} {arg_types : List LLType}
+  {defs : Definitions} (ctxRespectDefs : CtxRespectsDefs Γ defs)
+  (f : String) (h_args : Γ[f]? = some (LLType.func arg_types T_ret))
+  (f_in_defs : f ∈ defs) (eq_bd_defs : bd = defs[f].body)
+  : TypeJdg Γ (Expr.addBindings (ps.zip es) bd) T_ret
+    := by induction ps with
+      | nil =>
+        simp [Expr.addBindings]
+        let res := ctxRespectDefs T_ret arg_types f f_in_defs h_args
+        rw [eq_bd_defs.symm] at res
+        apply res
+      | cons head tail ih =>
+        sorry
+
 -- TODO: prove
 -- TODO: V and Γ should be related
 theorem preservation (Γ : TypeContext) (e e' : Expr) (ty : LLType) (defs : Definitions)
-    (h_env_respects : EnvRespectsCtx Γ V)
+    (h_env_respects : EnvRespectsCtx Γ V) (ctx_defs_respects : CtxRespectsDefs Γ defs)
   : TypeJdg Γ e ty → HeadSmallStep defs V e e' → TypeJdg Γ e' ty := by
   intro h_jdg b
   induction b
@@ -30,11 +54,6 @@ theorem preservation (Γ : TypeContext) (e e' : Expr) (ty : LLType) (defs : Defi
       cases H₂
       constructor
   · cases h_jdg
-    rename_i f es arg_types T_return h_f h_args
-    sorry
-
--- Progress: if TypeJdg Γ e ty, then e can take a step.
--- TODO: formalize
-
--- TODO: Also interesting:
--- if TypeJdg Γ e ty, then eval e succeeds
+    rename_i f es' ps bd f_in_defs a eq_bd_defs es eq arg_types h_f h_args
+    simp [es]
+    apply addBindings_typing ctx_defs_respects f h_args f_in_defs eq_bd_defs
